meta-theory/pure_alpha_equivScript.sml
@@ -100,6 +100,621 @@ Proof
   rw[closed_def,GSYM perm_exp_eqvt]
 QED
 
+
+
+
+
+
+        
+(**************** freevars/boundvars perm_exp lemmas ******************)
+
+Triviality perm1_MAP_set:
+ ∀ l.  set l DELETE x DELETE y ⊆ set (MAP (perm1 x y) l)
+Proof
+  Induct \\ fs[]
+  \\ strip_tac \\ rw[perm1_def]
+  \\ fs [EXTENSION,SUBSET_DEF] \\ metis_tac []
+QED
+
+Triviality subset_union_weakening_gen1:
+ A ⊆ x INSERT y INSERT B ⇒ A ⊆ x INSERT y INSERT (B ∪ C)
+Proof
+  fs [EXTENSION,SUBSET_DEF] \\ metis_tac []
+QED
+
+Triviality subset_union_weakening_gen2:
+ A ⊆ x INSERT y INSERT C ⇒ A ⊆ x INSERT y INSERT (B ∪ C)
+Proof
+  fs [EXTENSION,SUBSET_DEF] \\ metis_tac []
+QED
+
+Triviality Letrec_SUBSET_INSERT_DIFF_DISTRIBUTIVITY:
+  A ⊆ y INSERT x INSERT B ∪ D
+  ∧ E DELETE x DELETE y ⊆ C
+  ⇒
+  A DIFF C ⊆ y INSERT x INSERT ((B ∪ D) DIFF E)
+Proof
+  fs [EXTENSION,SUBSET_DEF] \\ metis_tac []
+QED
+
+Triviality subset_union_weakening:
+  A ⊆ B ⇒ (A ⊆ (B ∪ C))
+Proof
+  fs [EXTENSION,SUBSET_DEF] \\ metis_tac []
+QED
+
+Triviality DIFF_UNION_DISTRIBUTIVITY:
+  (A ∪ B) DIFF C = (A DIFF C) ∪ (B DIFF C)
+Proof
+  fs [EXTENSION,SUBSET_DEF] \\ metis_tac []
+QED
+
+Triviality  perm1_MAP_set2:
+ ∀ l. set (MAP (perm1 x y) l) DELETE x DELETE y ⊆ set l
+Proof
+  Induct \\ fs[]
+  \\ strip_tac \\ rw[perm1_def]
+  \\ fs [EXTENSION,SUBSET_DEF] \\ metis_tac []
+QED
+
+Theorem freevars_perm_exp_subset:
+  ∀ e. freevars (perm_exp x y e) ⊆ y INSERT x INSERT freevars e
+Proof
+  ho_match_mp_tac freevars_ind \\ rw[]
+  THEN1 (fs[perm_exp_def,perm1_def] \\ rw[])
+  THEN1 (
+    fs[perm_exp_def,perm1_def]
+    \\fs[MAP_MAP_o,combinTheory.o_DEF,LIST_TO_SET_FLAT]
+    \\ Induct_on ‘es’ \\ fs[]
+    \\ strip_tac \\ strip_tac
+    \\ fs[GSYM INSERT_UNION_EQ]
+    \\ rw[]
+    THEN1 (
+      irule subset_union_weakening \\ fs[]
+    )
+    \\ simp[INSERT_UNION_EQ]
+    \\ match_mp_tac (GEN_ALL subset_union_weakening_gen2) \\ fs[]
+  )
+  THEN1(
+    fs[perm_exp_def,perm1_def]
+    \\ conj_tac
+    \\ fs[EXTENSION,SUBSET_DEF] \\ metis_tac[]
+  )
+  THEN1(
+    fs[perm_exp_def,perm1_def,freevars_def]
+    \\ fs[] \\ rw[]
+    \\ fs [EXTENSION,SUBSET_DEF,MEM_FILTER] \\ TRY( metis_tac [])
+  )
+  THEN1(
+    fs[perm_exp_def]
+    \\ fs[FILTER_FLAT,FILTER_APPEND_DISTRIB,MAP_MAP_o,combinTheory.o_DEF]
+    \\ ‘(λx'. FST ((λ(x',z). (perm1 x y x',perm_exp x y z)) x')) =(perm1 x y) ∘ FST’ by (
+       fs[FUN_EQ_THM]
+       \\ Cases \\ fs[]
+    )
+    \\ fs[] \\ pop_assum kall_tac
+    \\ conj_tac
+    THEN1 (
+      fs[GSYM list_to_set_diff]
+      \\ match_mp_tac Letrec_SUBSET_INSERT_DIFF_DISTRIBUTIVITY \\ fs[]
+      \\ conj_tac
+      THEN1 ( match_mp_tac subset_union_weakening_gen1 \\ fs[])
+      \\ fs[GSYM MAP_MAP_o]
+      \\ fs[perm1_MAP_set]
+    )
+    \\ ‘(λx'. FILTER (λn. ¬MEM n (MAP (perm1 x y ∘ FST) lcs))
+                       ((λ(fn,e'). freevars e')
+                       ((λ(x',z). (perm1 x y x',perm_exp x y z)) x')))
+        =
+        FILTER (λn. ¬MEM n (MAP (perm1 x y ∘ FST) lcs))
+        ∘ freevars
+        ∘ (perm_exp x y)
+        ∘ SND ’ by (
+       fs[FUN_EQ_THM]
+       \\ Cases \\ rw[]
+    ) \\ fs[] \\ pop_assum kall_tac
+    \\ fs[MAP_FILTER]
+    \\ fs[GSYM MAP_MAP_o]
+    \\ fs[GSYM FILTER_FLAT]
+    \\ fs[GSYM list_to_set_diff]
+    \\ match_mp_tac Letrec_SUBSET_INSERT_DIFF_DISTRIBUTIVITY  \\ fs[]
+    \\ reverse (rw[]) THEN1 (fs[perm1_MAP_set])
+    \\ match_mp_tac subset_union_weakening_gen2 \\ fs[]
+    \\ fs[MAP_MAP_o,LIST_TO_SET_FLAT]
+    \\ fs[BIGUNION_SUBSET]
+    \\ fs[MEM_MAP]
+    \\ strip_tac \\ rw[]
+    \\ Cases_on ‘y'’ \\ fs[]
+    \\ match_mp_tac SUBSET_TRANS
+    \\ qexists_tac ‘ y INSERT x INSERT freevars r’
+    \\ conj_tac THEN1 (res_tac \\ fs[])
+    \\ fs[]
+    \\ res_tac
+    \\ ‘set (MAP (λ(fn,e). freevars e) lcs) = set (MAP set (MAP (freevars o SND) lcs))’by(
+      ntac 4 (pop_assum kall_tac)
+      \\ Induct_on ‘lcs’ \\ fs[]
+      \\ Cases \\ fs[]
+    )
+    \\ fs[] \\ pop_assum kall_tac
+    \\ fs[GSYM LIST_TO_SET_FLAT]
+    \\ fs[SUBSET_INSERT_DELETE]
+    \\ Induct_on ‘lcs’ \\ fs[MEM]
+    \\ rw[]
+    \\ res_tac \\ fs[]
+    \\ TRY (Cases_on ‘h’) \\ rw[]
+    \\ fs [EXTENSION,SUBSET_DEF] \\ metis_tac []
+  )
+QED
+
+Theorem freevars_perm_exp_subset_inv:
+  ∀e. freevars e ⊆ y INSERT x INSERT freevars (perm_exp x y e)
+Proof
+  ho_match_mp_tac freevars_ind \\ rw[]
+  THEN1 (fs[perm_exp_def,perm1_def] \\ rw[])
+  THEN1 (
+    fs[perm_exp_def,perm1_def]
+    \\fs[MAP_MAP_o,combinTheory.o_DEF,LIST_TO_SET_FLAT]
+    \\ Induct_on ‘es’ \\ fs[]
+    \\ strip_tac \\ strip_tac
+    \\ fs[GSYM INSERT_UNION_EQ]
+    \\ rw[]
+    THEN1 (
+      irule subset_union_weakening \\ fs[]
+    )
+    \\ simp[INSERT_UNION_EQ]
+    \\ fs[EXTENSION,SUBSET_DEF] \\ metis_tac[]
+  )
+  THEN1(
+    fs[perm_exp_def,perm1_def]
+    \\ fs[EXTENSION,SUBSET_DEF] \\ metis_tac[]
+  )
+  THEN1(
+    fs[perm_exp_def,perm1_def]
+    \\ fs[EXTENSION,SUBSET_DEF] \\ metis_tac[]
+  )
+  THEN1(
+    fs[perm_exp_def,perm1_def,freevars_def]
+    \\ fs[] \\ rw[]
+    \\ fs [EXTENSION,SUBSET_DEF,MEM_FILTER] \\ TRY( metis_tac [])
+  )
+  THEN1(
+    fs[perm_exp_def]
+    \\ fs[FILTER_FLAT,FILTER_APPEND_DISTRIB,MAP_MAP_o,combinTheory.o_DEF]
+    \\ ‘(λx'. FST ((λ(x',z). (perm1 x y x',perm_exp x y z)) x')) = (perm1 x y) ∘ FST’ by (
+       fs[FUN_EQ_THM]
+       \\ Cases \\ fs[]
+    )
+    \\ fs[] \\ pop_assum kall_tac
+    \\ ‘(λx'. FILTER (λn. ¬MEM n (MAP (perm1 x y ∘ FST) lcs))
+                       ((λ(fn,e'). freevars e')
+                       ((λ(x',z). (perm1 x y x',perm_exp x y z)) x')))
+        =
+        FILTER (λn. ¬MEM n (MAP (perm1 x y ∘ FST) lcs))
+        ∘ freevars
+        ∘ (perm_exp x y)
+        ∘ SND ’ by (
+       fs[FUN_EQ_THM]
+       \\ Cases \\ rw[]
+    ) \\ fs[] \\ pop_assum kall_tac
+    \\ fs[MAP_FILTER]
+    \\ fs[GSYM MAP_MAP_o]
+    \\ fs[GSYM FILTER_FLAT]
+    \\ fs[GSYM list_to_set_diff]
+    \\ fs[DIFF_UNION_DISTRIBUTIVITY]
+    \\ conj_tac
+    THEN1 (
+      fs[GSYM DIFF_UNION_DISTRIBUTIVITY]
+      \\ match_mp_tac Letrec_SUBSET_INSERT_DIFF_DISTRIBUTIVITY  \\ fs[]
+      \\ conj_tac
+      THEN1 (match_mp_tac subset_union_weakening_gen1 \\ fs[])
+      \\ fs[perm1_MAP_set2]
+    )
+    \\ fs[GSYM DIFF_UNION_DISTRIBUTIVITY]
+    \\ match_mp_tac Letrec_SUBSET_INSERT_DIFF_DISTRIBUTIVITY  \\ fs[]
+    \\ reverse (rw[]) THEN1 (fs[perm1_MAP_set2])
+    \\ match_mp_tac subset_union_weakening_gen2 \\ fs[]
+    \\ fs[MAP_MAP_o] \\ fs[GSYM LIST_TO_SET_FLAT]
+    \\ fs[BIGUNION_SUBSET]
+    \\ fs[MEM_MAP]
+    \\ fs[GSYM UNION_SUBSET]
+    \\ strip_tac \\ rw[]
+    \\ Cases_on ‘y'’ \\ fs[]
+    \\ res_tac
+    \\ match_mp_tac SUBSET_TRANS
+    \\ qexists_tac ‘ y INSERT x INSERT freevars (perm_exp x y r)’
+    \\ conj_tac THEN1 (fs [EXTENSION,SUBSET_DEF] \\ metis_tac[])
+    \\ fs[GSYM LIST_TO_SET_FLAT]
+    \\ fs[SUBSET_INSERT_DELETE]
+    \\ Induct_on ‘lcs’ \\ fs[MEM]
+    \\ rw[]
+    \\ res_tac \\ fs[]
+    \\ fs [EXTENSION,SUBSET_DEF] \\ metis_tac []
+  )
+QED
+
+Theorem freevar_perm_exp_MEM:
+ ∀ e. MEM x (freevars e) ⇒ MEM y (freevars (perm_exp x y e))
+Proof
+  ho_match_mp_tac freevars_ind
+  \\ rpt conj_tac
+  THEN1( fs[perm_exp_def,perm1_def] \\ rw[])
+  THEN1(
+     rw[] \\ fs[MEM_MAP] \\ rw[]
+     \\ res_tac
+     \\ fs[freevars_def,perm_exp_def,perm1_def]
+     \\ fs[MEM_FLAT]
+     \\ qexists_tac ‘(freevars (perm_exp x y e))’ \\ fs[]
+     \\ fs[MAP_MAP_o,combinTheory.o_DEF]
+     \\ fs[MEM_MAP]
+     \\ qexists_tac ‘e’ \\ fs[]
+  )
+  THEN1(rw[] \\ fs[perm_exp_def,perm1_def])
+  THEN1(
+    fs[perm_exp_def,perm1_def]
+    \\ rw[] \\ fs[MEM_FILTER]
+  )
+  THEN1(
+    rpt strip_tac
+    \\ fs[freevars_def,perm_exp_def,perm1_def]
+    THEN1 (
+      fs[MEM_FILTER]
+      \\ fs[MAP_MAP_o,combinTheory.o_DEF]
+      \\ CCONTR_TAC \\ fs[]
+      \\ fs[MEM_MAP]
+      \\ Cases_on ‘x'’ \\ fs[]
+      \\ Cases_on ‘q = x’ \\ fs[]
+      THEN1 (first_assum (qspec_then ‘(x,r)’ assume_tac) \\ fs[])
+      \\ Cases_on ‘q = y’ \\ fs[]
+   )
+   \\ fs[MEM_FILTER]
+   \\ fs[MAP_MAP_o,combinTheory.o_DEF]
+   \\ fs[MEM_MAP]
+   \\ CCONTR_TAC \\ fs[]
+   THEN1 (
+     Cases_on ‘x'’ \\ fs[]
+     \\ Cases_on ‘q = x’ \\ rw[] \\ fs[]
+     \\ first_assum (qspec_then ‘(q,r)’ assume_tac) \\ rw[] \\ fs[]
+     \\ Cases_on ‘q = y’ \\ fs[]
+   )
+   \\ rw[]
+   \\ fs[MEM_MAP]
+   \\ fs[MEM_FLAT]
+   \\ fs[MEM_MAP]
+   \\ Cases_on ‘y'’ \\ res_tac \\ fs[] \\ res_tac \\ fs[]
+   \\ first_x_assum (qspec_then ‘freevars (perm_exp x y r)’ assume_tac) \\ rw[] \\ fs[]
+   \\ first_x_assum (qspec_then ‘(q,r)’ assume_tac) \\ rw[] \\ fs[]
+  )
+QED
+
+Theorem freevar_perm_exp_not_MEM:
+ ∀ e. ¬MEM x (freevars e) ⇒ ¬ MEM y (freevars (perm_exp x y e))
+Proof
+  ho_match_mp_tac freevars_ind
+  \\ rpt conj_tac
+  THEN1( fs[perm_exp_def,perm1_def] \\ rw[])
+  THEN1(
+    rw[]
+    \\ fs[MEM_MAP]
+    \\ fs[freevars_def,perm_exp_def,perm1_def]
+    \\ fs[MEM_FLAT]
+    \\ fs[MAP_MAP_o,combinTheory.o_DEF]
+    \\ fs[MEM_MAP]
+    \\ CCONTR_TAC \\ fs[] \\ rw[]
+    \\ res_tac
+    \\ first_assum (qspec_then ‘set (freevars a)’ assume_tac)
+    \\ fs[] \\ fs[]
+    \\ pop_assum (qspec_then ‘a’ assume_tac) \\ fs[]
+  )
+  THEN1(rw[] \\ fs[perm_exp_def,perm1_def])
+  THEN1(
+    fs[perm_exp_def,perm1_def]
+    \\ rw[] \\ fs[MEM_FILTER]
+  )
+  THEN1(
+    fs[freevars_def,perm_exp_def,perm1_def]
+    \\ rw[]
+    THEN1 (
+      fs[MEM_FILTER,MEM_FLAT,MEM_MAP,MAP_MAP_o,combinTheory.o_DEF]
+      \\ CCONTR_TAC \\ fs[] \\ rw[] \\ fs[]
+      \\ Cases_on ‘y''’ \\ rw[] \\ fs[]
+      \\ res_tac
+      \\ Cases_on ‘MEM x (freevars r)’ \\ fs[]
+      \\ last_x_assum (qspec_then ‘freevars r’ assume_tac) \\ rw[] \\ fs[]
+      \\ pop_assum (qspec_then ‘(q,r)’ assume_tac) \\ rw[] \\ fs[]
+    )
+    \\ fs[GSYM perm1_def]
+    \\ fs[MEM_FILTER]
+    \\ fs[MAP_MAP_o,combinTheory.o_DEF] \\ rw[]
+    \\ disj1_tac
+    \\ ‘(λx'. FST ((λ(x',z). (perm1 x y x',perm_exp x y z)) x')) = (perm1 x y) o FST’ by (
+       fs[FUN_EQ_THM]
+       \\ Cases \\ rw[]
+    )
+    \\ fs[] \\ pop_assum kall_tac
+    \\ fs[MEM_MAP]
+    \\ qexists_tac ‘y'’ \\ fs[]
+    \\ Cases_on ‘y'’ \\ fs[perm1_def]
+  )
+QED
+
+Theorem freevars_perm_exp:
+  freevars (perm_exp x y e) =
+     freevars e
+     DIFF (if x ∉ freevars e then {y} else ∅)
+     DIFF (if y ∉ freevars e then {x} else ∅)
+     ∪ (if x ∈ freevars e then {y} else ∅)
+     ∪ (if y ∈ freevars e then {x} else ∅)
+Proof
+  rw[]
+  \\ assume_tac (GEN_ALL freevars_perm_exp_subset)
+  \\ assume_tac (GEN_ALL freevars_perm_exp_subset_inv)
+  \\ assume_tac (GEN_ALL freevar_perm_exp_MEM)
+  \\ assume_tac (GEN_ALL freevar_perm_exp_not_MEM)
+  \\ TRY (fs [EXTENSION,SUBSET_DEF] \\ metis_tac [perm_exp_sym])
+QED
+
+Theorem boundvars_perm_exp_subset:
+  ∀ e.
+  boundvars (perm_exp x y e) ⊆ x INSERT y INSERT (boundvars e)
+Proof
+  recInduct boundvars_ind
+  \\ rw[]
+  THEN1 (fs[perm_exp_def])
+  THEN1 (
+    fs[perm_exp_def]
+    \\ fs[MAP_MAP_o,combinTheory.o_DEF]
+    \\ fs[LIST_TO_SET_FLAT]
+    \\ fs[MAP_MAP_o,combinTheory.o_DEF]
+    \\ fs[MEM_MAP]
+    \\ fs[BIGUNION_SUBSET]
+    \\ rw[]
+    \\ fs[MEM_MAP]
+    \\ last_assum (qspec_then ‘a’ assume_tac)
+    \\ res_tac \\ fs[]
+    \\ irule SUBSET_TRANS
+    \\ qexists_tac ‘ x INSERT y INSERT boundvars a’
+    \\ fs[]
+    \\ irule SUBSET_INSERT_RIGHT
+    \\ irule SUBSET_INSERT_RIGHT
+    \\ irule SUBSET_BIGUNION_I
+    \\ fs[MEM_MAP]
+    \\ qexists_tac ‘a’ \\ fs[]
+  )
+  THEN1 (
+    fs[perm_exp_def]
+    \\ fs[DISJOINT_SYM]
+    \\ fs[EXTENSION,SUBSET_DEF] \\ metis_tac[]
+  )
+  THEN1 (
+    fs[perm_exp_def,boundvars_def,perm1_def]
+    \\ rw[]
+    \\ fs[EXTENSION,SUBSET_DEF] \\ metis_tac[]
+  )
+  \\ fs[perm_exp_def]
+  \\ reverse conj_tac
+  THEN1 (fs[EXTENSION,SUBSET_DEF] \\ metis_tac[])
+  \\ fs[MAP_MAP_o,combinTheory.o_DEF]
+  \\ fs[LIST_TO_SET_FLAT]
+  \\ fs[MAP_MAP_o,combinTheory.o_DEF]
+  \\ fs[MEM_MAP]
+  \\ fs[BIGUNION_SUBSET]
+  \\ rw[]
+  \\ fs[MEM_MAP]
+  \\ Cases_on ‘x'’
+  \\ fs[perm1_def]
+  \\ reverse conj_tac
+  THEN1 (
+     rw[]
+     \\ res_tac
+     \\ irule SUBSET_TRANS
+     \\ qexists_tac ‘x INSERT y INSERT
+                     BIGUNION (set (MAP (λ(fn,e). fn INSERT boundvars e) lcs))’
+     \\ reverse conj_tac
+     THEN1 (fs[EXTENSION,SUBSET_DEF,UNION_DEF] \\ metis_tac[])
+     \\ fs[SUBSET_INSERT_DELETE]
+     \\ irule SUBSET_TRANS
+     \\ qexists_tac ‘q INSERT boundvars r’
+     \\ conj_tac
+     THEN1 (fs[EXTENSION,SUBSET_DEF,UNION_DEF] \\ metis_tac[])
+     \\ irule SUBSET_BIGUNION_I
+     \\ fs[MEM_MAP]
+     \\ qexists_tac ‘(q,r)’ \\ fs[]
+  )
+  \\ rw[]
+  \\ disj2_tac
+  \\ qexists_tac ‘q INSERT boundvars r’
+  \\ fs[]
+  \\ fs[MEM_MAP]
+  \\ qexists_tac ‘(q,r)’ \\ fs[]
+QED
+
+Theorem boundvars_perm_exp_subset_inv:
+  ∀e. boundvars e ⊆ x INSERT y INSERT boundvars (perm_exp x y e)
+Proof
+  recInduct boundvars_ind
+  \\ rw[]
+  THEN1 (
+    fs[perm_exp_def]
+    \\ fs[MAP_MAP_o,combinTheory.o_DEF]
+    \\ fs[LIST_TO_SET_FLAT]
+    \\ fs[MAP_MAP_o,combinTheory.o_DEF]
+    \\ fs[MEM_MAP]
+    \\ fs[BIGUNION_SUBSET]
+    \\ rw[]
+    \\ fs[MEM_MAP]
+    \\ res_tac
+    \\ irule SUBSET_TRANS
+    \\ qexists_tac ‘ x INSERT y INSERT boundvars (perm_exp x y e)’
+    \\ fs[]
+    \\ irule SUBSET_INSERT_RIGHT
+    \\ irule SUBSET_INSERT_RIGHT
+    \\ irule SUBSET_BIGUNION_I
+    \\ fs[MEM_MAP]
+    \\ qexists_tac ‘e’ \\ fs[]
+  )
+  THEN1 (
+    fs[perm_exp_def]
+    \\ fs[EXTENSION,SUBSET_DEF] \\ metis_tac[]
+  )
+  THEN1 (
+    fs[perm_exp_def]
+    \\ fs[EXTENSION,SUBSET_DEF] \\ metis_tac[]
+  )
+  THEN1 (
+    fs[perm_exp_def]
+    \\ fs[perm1_def]
+    \\ rw[]
+  )
+  THEN1 (
+    fs[perm_exp_def]
+    \\ fs[perm1_def]
+    \\ rw[]
+    \\ fs[EXTENSION,SUBSET_DEF] \\ metis_tac[]
+  )
+  THEN1 (
+    fs[perm_exp_def]
+    \\ fs[MAP_MAP_o,combinTheory.o_DEF]
+    \\ fs[LIST_TO_SET_FLAT]
+    \\ fs[MAP_MAP_o,combinTheory.o_DEF]
+    \\ fs[EXTENSION,UNION_DEF,SUBSET_DEF] \\ metis_tac[]
+  )
+  \\ fs[perm_exp_def]
+  \\ fs[MAP_MAP_o,combinTheory.o_DEF]
+  \\ fs[LIST_TO_SET_FLAT]
+  \\ fs[MAP_MAP_o,combinTheory.o_DEF]
+  \\ fs[BIGUNION_SUBSET]
+  \\ rw[]
+  \\ fs[MEM_MAP]
+  \\ Cases_on ‘y'’
+  \\ fs[perm1_def]
+  \\ rw[]
+  THEN1 (
+    CCONTR_TAC \\ fs[] \\ res_tac \\ fs[MEM_MAP]
+    \\ first_assum (qspec_then ‘q INSERT (boundvars (perm_exp x y r))’ assume_tac) \\ fs[]
+    \\ first_assum (qspec_then ‘(q,r)’ assume_tac) \\ fs[]
+    \\ pop_assum mp_tac \\ rw[]
+  )
+  \\ res_tac
+  \\ fs[SUBSET_INSERT_DELETE]
+  \\ irule SUBSET_TRANS
+  \\ qexists_tac ‘perm1 x y q INSERT boundvars (perm_exp x y r)’
+  \\ conj_tac THEN1 (fs[EXTENSION,SUBSET_DEF] \\ metis_tac[])
+  \\ irule subset_union_weakening
+  \\ irule SUBSET_BIGUNION_I
+  \\ fs[MEM_MAP]
+  \\ qexists_tac ‘(q,r)’ \\ fs[perm1_def] \\ rw[]
+QED
+
+Theorem boundvar_perm_exp_MEM:
+ ∀ e. MEM x (boundvars e) ⇒ MEM y (boundvars (perm_exp x y e))
+Proof
+  ho_match_mp_tac boundvars_ind
+  \\ rw[]
+  \\ fs[perm_exp_def]
+  \\ fs[perm1_def]
+  THEN1 (
+    fs[MAP_MAP_o,combinTheory.o_DEF]
+    \\ fs[MEM_FLAT]
+    \\ fs[MEM_MAP]
+    \\ rw[]
+    \\ res_tac
+    \\ qexists_tac ‘boundvars (perm_exp x y e)’
+    \\ rw[]
+    \\ qexists_tac ‘e’
+    \\ fs[]
+  )
+  \\ fs[GSYM perm1_def]
+  \\ fs[MAP_MAP_o,combinTheory.o_DEF]
+  \\ fs[MEM_FLAT]
+  \\ fs[MEM_MAP]
+  \\ rw[]
+  \\ Cases_on ‘y'’
+  \\ res_tac \\ fs[] \\ rw[]
+  THEN1 (
+    disj1_tac
+    \\ qexists_tac ‘y::(boundvars (perm_exp q y r))’
+    \\ fs[] \\ rw[]
+    \\ qexists_tac ‘(q,r)’
+    \\ fs[] \\ rw[]
+    \\ fs[perm1_def]
+  )
+  \\ res_tac \\ fs[] \\ rw[]
+  \\ disj1_tac
+  \\ Cases_on ‘MEM y (boundvars (perm_exp x y e))’ \\ fs[]
+  \\ qexists_tac ‘perm1 x y q::(boundvars (perm_exp x y r))’
+  \\ fs[] \\ rw[]
+  \\ qexists_tac ‘(q,r)’
+  \\ fs[] \\ rw[]
+QED
+
+Theorem boundvar_perm_exp_not_MEM:
+ ∀ e. ¬MEM x (boundvars e) ⇒ ¬ MEM y (boundvars (perm_exp x y e))
+Proof
+  ho_match_mp_tac boundvars_ind
+  \\ rw[]
+  \\ fs[perm_exp_def]
+  \\ fs[perm1_def]
+  THEN1 (
+    fs[MAP_MAP_o,combinTheory.o_DEF]
+    \\ fs[MEM_FLAT]
+    \\ fs[MEM_MAP]
+    \\ CCONTR_TAC \\ fs[]
+    \\ res_tac \\ rw[]
+    \\ Cases_on ‘MEM x (boundvars a)’ \\ fs[]
+    \\ first_assum (qspec_then ‘boundvars a’ assume_tac) \\ fs[] \\ fs[]
+    \\ metis_tac[]
+  )
+  THEN1 (
+    IF_CASES_TAC \\ fs[]
+  )
+  \\ fs[GSYM perm1_def]
+  \\ fs[MAP_MAP_o,combinTheory.o_DEF]
+  \\ fs[MEM_FLAT]
+  \\ fs[MEM_MAP]
+  \\ rw[]
+  \\ CCONTR_TAC \\ fs[]
+  \\ Cases_on ‘x'’ \\ fs[] \\ rw[]
+  \\ res_tac \\ fs[] \\ rw[]
+  THEN1 (
+    fs[perm1_def]
+    \\ pop_assum mp_tac
+    \\ pop_assum mp_tac
+    \\ IF_CASES_TAC \\ fs[]
+    \\ rw[] \\ res_tac \\ fs[]
+    \\ first_assum (qspec_then ‘q INSERT boundvars r’ assume_tac) \\ fs[]
+    \\ first_assum (qspec_then ‘(q,r)’ assume_tac) \\ fs[]
+  )
+  \\ Cases_on ‘MEM x (boundvars r)’ \\ fs[]
+  \\ first_assum (qspec_then ‘q INSERT boundvars r’ assume_tac) \\ fs[]
+  \\ fs[] \\ rw[]
+  \\ first_assum (qspec_then ‘(q,r)’ assume_tac) \\ fs[]
+QED
+
+Theorem boundvars_perm_exp:
+  boundvars (perm_exp x y e) =
+     boundvars e
+     DIFF (if x ∉ boundvars e then {y} else ∅)
+     DIFF (if y ∉ boundvars e then {x} else ∅)
+     ∪ (if x ∈ boundvars e then {y} else ∅)
+     ∪ (if y ∈ boundvars e then {x} else ∅)
+Proof
+  rw[]
+  \\ assume_tac (GEN_ALL boundvars_perm_exp_subset)
+  \\ assume_tac (GEN_ALL boundvars_perm_exp_subset_inv)
+  \\ assume_tac (GEN_ALL boundvar_perm_exp_MEM)
+  \\ assume_tac (GEN_ALL boundvar_perm_exp_not_MEM)
+  \\ fs [EXTENSION,SUBSET_DEF] \\ metis_tac [perm_exp_sym]
+QED
+
+
+(*******************)
+
+
+
+        
+
+        
+
 Definition perm_v_def:
   perm_v x y v =
   gen_v (λpath.
